src/robots/car/firstQuadrant.v
@@ -1,0 +1,290 @@
+(** printing × $\times$ #×# *)
+(** printing :> $:$ #:># *)
+(** printing ≡ $\equiv$ #≡# *)
+(** printing [*] $*$ #*# *)
+(** printing ∧ $\wedge$ #∧# *)
+(** printing ∀ $\forall$ #∀# *)
+(** printing → $\rightarrow$ #→# *)
+(** printing ∃ $\exists$ #∃# *)
+(** printing ≤ $\le$ #≤# *)
+(** printing θ $\theta$ #θ# *)
+(** printing eeev $\epsilon_v$ #∊ᵥ# *)
+(** printing eeew $\epsilon_w$ #∊w# *)
+(** printing tm $t_m$ #tm# *)
+(** printing IR $\mathbb{R}$ #IR# *)
+(** printing CR $\mathbb{R}$ #CR# *)
+(** printing tr $t_r$ #tr# *)
+(** remove printing * *)
+
+(** printing ' $ $ #'# *)
+
+Require Import Vector.
+
+Require Import MathClasses.interfaces.canonical_names.
+Require Import MCInstances.
+Require Import ackermannSteering.
+Require Import MCMisc.tactics.
+Require Import CartIR.
+Require Import ackermannSteering.
+Require Import fastReals.interface.
+Require Import fastReals.misc.
+Require Import geometry2D.
+Require Import geometry2DProps.
+Require Import ackermannSteeringProp.
+Require Import MathClasses.orders.rings.
+Require Import MathClasses.interfaces.orders.
+Require Import ackermannSteeringProp.
+Require Import IRMisc.LegacyIRRing.
+
+
+Local Opaque CSine.
+Local Opaque CCos.
+Local Opaque Sine.
+Local Opaque Cosine.
+Local Opaque Sin.
+Local Opaque Cos.
+
+
+  Local Notation minxy := (lstart).
+  Local Notation maxxy := (lend).
+  Local Notation  "∫" := Cintegral.
+  
+(** Many trignometric comparisons can be made easily
+if the angles are in a fixed quadrant
+For getting in/out of a parallel parked spot, a car's orientation does not
+need to change by 90 degrees, even though the car moves
+both forward and backward. So we assume that its
+orientation remains in the first quadrant (between 0 and 90).
+Assume that the X axis represents the road.
+Now, it is easy to characterize the X Y extent of the car,
+in terms of the coordinates of the four corners of the car*)
+Section Rigid2DState.
+  Variable cs :Rigid2DState IR.
+  Variable cd :CarDimensions IR.
+  Hypothesis nonTriv : nonTrivialCarDim cd.
+  Hypothesis theta90 : 0 ≤ θ2D cs ≤ (½ * π).
+  
+  Lemma carBoundsAMAuxMin : 
+    minCart (rightSideUnitVec cs * ' width cd) (- (rightSideUnitVec cs * ' width cd))
+    = -('width cd) * {|X:= sin (θ2D cs); Y:= cos (θ2D cs)|}.
+  Proof using All.
+    destruct nonTriv as [a b]. destruct b as [c b].
+    apply unitVecNonNeg in theta90.
+    unfold unitVec in theta90.
+    destruct theta90 as [x y]. simpl in x, y.
+    apply less_leEq in c.
+    unfold rightSideUnitVec. rewrite unitVecMinus90.
+    unfold minCart. split; simpl;
+    autounfold with IRMC.
+    - rewrite Min_comm.
+      rewrite leEq_imp_Min_is_lft;[ring|].
+      rewrite <- cring_inv_mult_rht.
+      apply mult_resp_leEq_rht;[| assumption].
+      apply shift_leEq_rht. unfold cg_minus.
+      rewrite cg_inv_inv.
+      apply plus_resp_nonneg; assumption.
+
+    - rewrite leEq_imp_Min_is_lft;[ring|].
+      rewrite  cring_inv_mult_rht.
+      apply inv_resp_leEq.
+      rewrite <- cring_inv_mult_rht.
+      apply mult_resp_leEq_rht;[| assumption].
+      apply shift_leEq_rht. unfold cg_minus.
+      rewrite cg_inv_inv.
+      apply plus_resp_nonneg; assumption.
+  Qed.
+
+  (* only needed to replace leEq_imp_Min_is_lft by leEq_imp_Max_is_rht *)
+  Lemma carBoundsAMAuxMax : 
+    maxCart (rightSideUnitVec cs * ' width cd) (- (rightSideUnitVec cs * ' width cd))
+    = ('width cd) * {|X:= sin (θ2D cs); Y:= cos (θ2D cs)|}.
+  Proof using All.
+    destruct nonTriv as [a b]. destruct b as [c b].
+    apply unitVecNonNeg in theta90.
+    unfold unitVec in theta90.
+    destruct theta90 as [x y]. simpl in x, y.
+    apply less_leEq in c.
+    unfold rightSideUnitVec. rewrite unitVecMinus90.
+    unfold maxCart. split; simpl;
+    autounfold with IRMC.
+    - rewrite Max_comm.
+      rewrite leEq_imp_Max_is_rht;[ring|].
+      rewrite <- cring_inv_mult_rht.
+      apply mult_resp_leEq_rht;[| assumption].
+      apply shift_leEq_rht. unfold cg_minus.
+      rewrite cg_inv_inv.
+      apply plus_resp_nonneg; assumption.
+
+    - rewrite leEq_imp_Max_is_rht;[ring|].
+      rewrite  cring_inv_mult_rht.
+      apply inv_resp_leEq.
+      rewrite <- cring_inv_mult_rht.
+      apply mult_resp_leEq_rht;[| assumption].
+      apply shift_leEq_rht. unfold cg_minus.
+      rewrite cg_inv_inv.
+      apply plus_resp_nonneg; assumption.
+  Qed.
+
+  Lemma carBoundsAMAuxMin2 : 
+    minCart 
+      ((- frontUnitVec cs * ' lengthBack cd)) 
+      (frontUnitVec cs * ' lengthFront cd)
+    =  -(frontUnitVec cs) * (' lengthBack cd).
+  Proof using All.
+    rewrite <- negate_mult_distr_l.
+    rewrite negate_mult_distr_r.
+    unfold frontUnitVec.
+    setoid_rewrite <- sameXYNegate.
+    setoid_rewrite unitVecMinDistr;[| assumption].
+    fequiv.
+    unfold cast, castCRCart2DCR. 
+    fequiv.
+    apply leEq_imp_Min_is_lft.
+    apply shift_leEq_rht.
+    unfold cg_minus. revert nonTriv.
+    unfold nonTrivialCarDim.
+    autounfold with IRMC.
+    intros.
+    rewrite cg_inv_inv.
+      apply plus_resp_nonneg; tauto.
+  Qed.
+
+  Lemma carBoundsAMAuxMax2 : 
+    maxCart 
+      ((- frontUnitVec cs * ' lengthBack cd)) 
+      (frontUnitVec cs * ' lengthFront cd)
+    =  (frontUnitVec cs) * (' lengthFront cd).
+  Proof using All.
+    rewrite <- negate_mult_distr_l.
+    rewrite negate_mult_distr_r.
+    unfold frontUnitVec.
+    setoid_rewrite <- sameXYNegate.
+    setoid_rewrite unitVecMaxDistr;[| assumption].
+    fequiv.
+    fequiv.
+    apply leEq_imp_Max_is_rht.
+    apply shift_leEq_rht.
+    unfold cg_minus. revert nonTriv.
+    unfold nonTrivialCarDim.
+    autounfold with IRMC.
+    intros.
+    rewrite cg_inv_inv.
+      apply plus_resp_nonneg; tauto.
+  Qed.
+    
+  Lemma carBoundsAMAux : carMinMaxXY cd cs =
+  {|minxy := {|X:= X (backLeft cd cs); Y:= Y (backRight cd cs)|};
+     maxxy := {|X:= X (frontRight cd cs); Y:= Y (frontLeft cd cs) |} |}.
+  Proof using All.
+  unfold carMinMaxXY.
+  unfold backRight, backLeft.
+  Local Opaque unitVec.
+  simpl. unfold  boundingUnion.
+  simpl. 
+  Typeclasses eauto :=10.
+  pose proof (minCartSum (pos2D cs - frontUnitVec cs * ' lengthBack cd)).
+  unfold BoundingRectangle. simpl.
+  Local Opaque minCart.
+  Local Opaque maxCart.
+  simpl. split; simpl.
+  - rewrite  (@simple_associativity _ _ (@plus (Cart2D IR) _) _ _).
+    rewrite  (@simple_associativity _ _ (@plus (Cart2D IR) _) _ _).  
+    rewrite (minCartSum _).
+    rewrite carBoundsAMAuxMin.
+    rewrite <- (@simple_associativity _ _ (@minCart IR _) _ _).
+    unfold frontRight, frontLeft.
+    rewrite  (@simple_associativity _ _ (@plus (Cart2D IR) _) _ _).
+    rewrite  (@simple_associativity _ _ (@plus (Cart2D IR) _) _ _).  
+    rewrite minCartSum.
+    rewrite (@commutativity _ _ _ (@minCart IR _) _ _ (rightSideUnitVec cs * ' width cd)).
+    rewrite carBoundsAMAuxMin.
+    rewrite <- (@simple_associativity _ _ (@plus (Cart2D IR) _) _ _).
+    rewrite <- (@simple_associativity _ _ (@plus (Cart2D IR) _) _ _).
+    rewrite minCartSum.
+    rewrite (@commutativity _ _ _ (@plus (Cart2D IR) _) _ _ 
+      (-' width cd * {| X := sin (θ2D cs); Y := cos (θ2D cs) |})).
+    rewrite (@commutativity _ _ _ (@plus (Cart2D IR) _) _ _ 
+      (-' width cd * {| X := sin (θ2D cs); Y := cos (θ2D cs) |})).
+    rewrite minCartSum. simpl.
+    rewrite carBoundsAMAuxMin2.
+    unfold rightSideUnitVec. rewrite unitVecMinus90.
+    split; simpl; autounfold with IRMC; IRring.
+  - 
+    rewrite  (@simple_associativity _ _ (@plus (Cart2D IR) _) _ _).
+    rewrite  (@simple_associativity _ _ (@plus (Cart2D IR) _) _ _).  
+      rewrite (maxCartSum _).
+    rewrite carBoundsAMAuxMax.
+    rewrite <- (@simple_associativity _ _ (@maxCart IR _) _ _).
+    unfold frontRight, frontLeft.
+    rewrite  (@simple_associativity _ _ (@plus (Cart2D IR) _) _ _).
+    rewrite  (@simple_associativity _ _ (@plus (Cart2D IR) _) _ _).  
+    rewrite maxCartSum.
+    rewrite (@commutativity _ _ _ (@maxCart IR _) _ _ (rightSideUnitVec cs * ' width cd)).
+    rewrite carBoundsAMAuxMax.
+    rewrite <- (@simple_associativity _ _ (@plus (Cart2D IR) _) _ _).
+    rewrite <- (@simple_associativity _ _ (@plus (Cart2D IR) _) _ _).
+    rewrite maxCartSum.
+    rewrite (@commutativity _ _ _ (@plus (Cart2D IR) _) _ _ 
+      (' width cd * {| X := sin (θ2D cs); Y := cos (θ2D cs) |})).
+    rewrite (@commutativity _ _ _ (@plus (Cart2D IR) _) _ _ 
+      (' width cd * {| X := sin (θ2D cs); Y := cos (θ2D cs) |})).
+    rewrite maxCartSum.
+    rewrite carBoundsAMAuxMax2.
+    unfold rightSideUnitVec. rewrite unitVecMinus90.
+    split; simpl; autounfold with IRMC; IRring.
+  Qed.
+
+
+  (** When the turn curvature is fixed, a car's position and orientation, and hence
+   the position of its corners, and hence the confining axis-aligned rectangle,
+   can be defined just as a function of initial state and the car's orientation.
+    The lemma [carMinMaxXYAM] below proves the correctness of this definition..
+  *)
+   
+  Definition carMinMaxXYAtθ  (init : Rigid2DState IR) (cd : CarDimensions IR)
+        (turnRadius θ : IR) : Line2D IR :=  
+  let θi := θ2D init in
+  '(pos2D init) +
+  {| minxy:= {|
+      X := turnRadius * (sin θ - sin θi) - (width cd) * sin θ - (lengthBack cd) * cos  θ;
+      Y := turnRadius * (cos θi - cos θ) - (width cd) * cos θ - (lengthBack cd) * sin  θ
+        |};
+     maxxy := {|
+      X := turnRadius * (sin θ - sin θi) + (width cd) * sin θ + (lengthFront cd) * cos  θ;
+      Y := turnRadius * (cos θi - cos θ) + (width cd) * cos θ + (lengthFront cd) * sin  θ
+        |}
+  |}.
+  
+  Global Instance ProperCarMinMaxAtθ : Proper
+    (equiv ==> equiv ==> equiv ==> equiv ==> equiv) 
+       carMinMaxXYAtθ.
+  Proof using.
+    intros ? ? H1e ? ? H2e ? ? H3e ? ? H4e.
+    unfold carMinMaxXYAtθ. rewrite H1e.
+    rewrite H2e. rewrite H3e.  rewrite H4e.
+    reflexivity.
+  Qed.
+End Rigid2DState.
+
+Section TurnMove.
+  Variable cd :CarDimensions IR.
+  Hypothesis nonTriv : nonTrivialCarDim cd.
+  
+  Lemma carMinMaxXYAM : forall init tr θ,
+  (0 ≤ θ ≤ (½ * π))
+  ->
+    carMinMaxXY cd (turnRigidStateAtθ init tr θ)
+    = carMinMaxXYAtθ init cd tr θ.
+  Proof using nonTriv.
+    intros ? ? ? H90.
+    rewrite carBoundsAMAux;[| assumption | exact H90].
+    Local Opaque unitVec.
+      simpl. unfold rightSideUnitVec.
+      rewrite unitVecMinus90.
+    Local Transparent unitVec. simpl. 
+    rewrite foldPlusCart.
+    split;split; simpl;
+    IRring.
+  Qed.
+
+End TurnMove.
